misc

nominal_machine.lean
@@ -1,22 +1,11 @@
-import data.hash_map
+import data.hash_map .atom
 
 namespace nominal
 open list
 
-structure atom := (id : nat)
-namespace atom
-instance : decidable_eq atom := by tactic.mk_dec_eq_instance
-
-end atom
-
-def fresh_atom_core : list atom → ℕ → atom
-| [] next_id := ⟨next_id⟩
-| (atom::atoms) next_id := fresh_atom_core atoms (max atom^.id next_id)
-
-def fresh_atom (atoms : list atom) : atom := fresh_atom_core atoms 0
-
 inductive exp : Type
 | var : atom → exp
+| const : ℕ → exp
 | abs : atom → exp → exp
 | app : exp → exp → exp
 
@@ -24,6 +13,7 @@ open exp
 
 def fvs : exp → list atom
 | (var v)     := [v]
+| (const n)   := []
 | (abs v e)   := remove_all (fvs e) [v]
 | (app e₁ e₂) := fvs e₁ ∪ fvs e₂
 
@@ -32,26 +22,27 @@ def swap_var (x y z : atom) : atom :=
 
 def swap (x y : atom) : exp → exp
 | (var z)     := var (swap_var x y z)
+| (const n)   := const n
 | (abs z e)   := abs (swap_var x y z) (swap e)
 | (app e₁ e₂) := app (swap e₁) (swap e₂)
 
-def heap := hash_map atom (λ x, exp)
+@[reducible] def heap := hash_map atom (λ x, exp)
 structure frame := (val : exp)
 def stack := list frame
 
 structure config := (hp : heap) (t : exp) (stk : stack)
 
 inductive step (α : Type) : Type
-| error {} : step
-| done  {} : step
-| take     : α → step
+| error {}  : step
+| done  {}  : exp → step
+| take      : α → step
 
 def machine_step (avoid : list atom) : config → step config
-| ⟨hp, abs x e, []⟩ := step.done
+| ⟨hp, abs x e, []⟩ := step.done (abs x e)
 
 | ⟨hp, abs x e, (⟨val⟩ :: stk)⟩ :=
- if x ∈ hp^.keys ∪ avoid
- then let y := fresh_atom (hp^.keys ∪ avoid) in step.take ⟨hp^.insert y val, swap x y e, stk⟩
+ if x ∈ hp ∨ x ∈ avoid
+ then let y := atom.fresh (hp^.keys ∪ avoid) in step.take ⟨hp^.insert y val, swap x y e, stk⟩
  else step.take ⟨hp^.insert x val, e, stk⟩
 
 | ⟨hp, var x, stk⟩ := match hp^.find x with
@@ -61,19 +52,24 @@ def machine_step (avoid : list atom) : config → step config
 
 | ⟨hp, app f a, stk⟩ := step.take ⟨hp, f, ⟨a⟩ :: stk⟩
 
+
+| ⟨hp, const n, stk⟩ := step.done (const n)
+
 def init_config (t : exp) : config := ⟨mk_hash_map (λ a : atom, a^.id), t, []⟩
 
 def is_val : exp → Prop
 | (abs _ _) := true
 | _         := false
 
-lemma values_are_done (avoid : list atom) : ∀ (t : exp), is_val t → machine_step avoid (init_config t) = step.done
+lemma values_are_done (avoid : list atom) : ∀ (t : exp), is_val t → machine_step avoid (init_config t) = step.done t
 | (abs x e) _ := rfl
+| (const n) _ := rfl
 | (var v) H_contra := false.rec _ H_contra
 | (app f a) H_contra := false.rec _ H_contra
 
 def size : exp → ℕ
 | (var x) := 1
+| (const n) := 1
 | (abs x e) := 1 + size e
 | (app f a) := 1 + size f + size a
 
@@ -82,10 +78,45 @@ begin
 intro t,
 induction t,
 reflexivity,
-all_goals { simp [swap, size], cc }
+all_goals { simp [swap, size], try { cc } }
 end
 
+/-
+inductive exp : Type
+| var : atom → exp
+| const : ℕ → exp
+| abs : atom → exp → exp
+| app : exp → exp → exp
+-/
+open exp
 
+inductive result : Type
+| error   : string → result
+| done    : exp → result
+| nofuel  : exp → result
+
+def reduce (avoid : list atom) : ℕ → config → result
+| 0     ⟨hp, e, stk⟩       := result.nofuel e
+| (t+1) ⟨hp, abs x e, []⟩  := result.done (abs x e)
+| (t+1) ⟨hp, const n, stk⟩ := result.done (const n)
+
+| (t+1) ⟨hp, abs x e, (⟨val⟩ :: stk)⟩ :=
+ if x ∈ hp ∨ x ∈ avoid
+ then let y := atom.fresh (hp^.keys ∪ avoid) in reduce t ⟨hp^.insert y val, swap x y e, stk⟩
+ else reduce t ⟨hp^.insert x val, e, stk⟩
+
+| (t+1) ⟨hp, var x, stk⟩ :=
+ match hp^.find x with
+ | some e := reduce t ⟨hp, e, stk⟩
+ | none   := result.error "variable not found"
+ end
+
+| (t+1) ⟨hp, app f a, stk⟩ := reduce t ⟨hp, f, ⟨a⟩ :: stk⟩
+
+example : reduce [] 10 (init_config $ app (abs ⟨0⟩ (var ⟨0⟩)) (const 5)) = result.done (const 5) :=
+begin
+simp [reduce, init_config, hash_map.not_contains_empty, has_mem.mem, list.mem, hash_map.find_insert],
+end
 
 
 
