atom.lean
@@ -1,0 +1,11 @@
+structure atom := (id : nat)
+namespace atom
+instance : decidable_eq atom := by tactic.mk_dec_eq_instance
+
+def fresh_atom_core : list atom → ℕ → atom
+| [] next_id := ⟨next_id⟩
+| (atom::atoms) next_id := fresh_atom_core atoms (max atom^.id next_id)
+
+def fresh (atoms : list atom) : atom := fresh_atom_core atoms 0
+
+end atom
