locally_nameless.lean
@@ -1,0 +1,75 @@
+import .atom data.hash_map
+
+namespace locally_nameless
+
+inductive type : Type
+| base : type
+| arrow : type → type → type
+
+inductive exp : Type
+| var_b : ℕ → exp
+| var_f : atom → exp
+| const : ℕ → exp
+| abs   : exp → exp
+| app   : exp → exp → exp
+
+open exp
+
+def subst_exp (v:atom) (s:exp) : exp → exp
+| (var_b n)   := var_b n
+| (var_f x)   := if x = v then s else var_f x
+| (const n)  := const n
+| (abs e)     := abs (subst_exp e)
+| (app e₁ e₂) := app (subst_exp e₁) (subst_exp e₂)
+
+def fv_exp : exp → list atom
+| (var_b nat) := []
+| (var_f x)   := [x]
+| (const n)   := []
+| (abs e)     := fv_exp e
+| (app e₁ e₂) := fv_exp e₁ ∪ fv_exp e₂
+
+def open_exp_wrt_exp_core : ℕ → exp → exp → exp
+| k s (var_b n) := match has_ordering.cmp n k with
+               | ordering.lt  := var_b n
+               | ordering.eq  := s
+               | ordering.gt  := var_b (n-1)
+               end
+
+| k s (var_f x)   := var_f x
+| k s (const n)   := const n
+| k s (abs e)     := abs (open_exp_wrt_exp_core (k+1) s e)
+| k s (app e₁ e₂) := app (open_exp_wrt_exp_core k s e₁) (open_exp_wrt_exp_core k s e₂)
+
+
+def open_exp_wrt_exp (s e : exp) : exp := open_exp_wrt_exp_core 0 s e.
+
+def context : Type := hash_map atom (λ a, exp)
+
+def reduce : exp → option exp
+| (app (abs f) a) := have exp.sizeof (open_exp_wrt_exp a f) < exp.sizeof f + (exp.sizeof a + 2), from sorry, reduce (open_exp_wrt_exp a f)
+| (abs e)         := some (abs e)
+| (const n)       := some (const n)
+| (app _ _)       := none
+| (var_b n)       := none
+| (var_f v)       := none
+
+#check @reduce.equations._eqn_1
+#check @reduce.equations._eqn_2
+#check @reduce.equations._eqn_3
+#check @reduce.equations._eqn_4
+#check @reduce.equations._eqn_5
+#check @reduce.equations._eqn_6
+#check @reduce.equations._eqn_7
+#check @reduce.equations._eqn_8
+
+lemma not_lt_refl : ∀ (n : ℕ), ¬ (n < n) := sorry
+
+example : reduce (app (abs (var_b 0)) (const 5)) = some (const 5) :=
+begin
+simp [reduce, open_exp_wrt_exp, open_exp_wrt_exp_core, open_exp_wrt_exp_core._match_1, has_ordering.cmp, nat.cmp, not_lt_refl],
+end
+
+
+
+end locally_nameless
